HolBA/src/tools/parallelcomposition/instantiations/bir_comp_attacker_vs_sbir_comp_DYScript.sml
@@ -4,10 +4,10 @@ open pred_setTheory;
 open sigma_algebraTheory;
 open listTheory;
 open tautLib;
-open interleavinggeneraldeductionTheory;
-open parallelcompositiongeneraldeductionTheory;
+open interleavingdeductionTheory;
+open parallelcompositiondeductionTheory;
 open translate_to_sapicTheory;
-open derived_rules_generaldeductionTheory;
+open derived_rules_deductionTheory;
 open sbir_treeTheory;
 open sapicplusTheory;
 open messagesTheory;
@@ -33,14 +33,14 @@ val att_traces_def = Define `
 `;
     
 val sbir_traces_thm =
-INST_TYPE [``:'symb`` |-> ``:Var_t``,``:'pred`` |-> ``:'SPpred``,``:'state`` |-> ``:(sbir_event, real,(bir_var_t, bir_exp_t) symb_interpret_t) stree``,``:'event`` |-> ``:(sbir_event + (Name_t, Var_t) sync_event)``] derived_rules_generaldeductionTheory.traces_def;
+INST_TYPE [``:'symb`` |-> ``:Var_t``,``:'pred`` |-> ``:'SPpred``,``:'state`` |-> ``:(sbir_event, real,(bir_var_t, bir_exp_t) symb_interpret_t) stree``,``:'event`` |-> ``:(sbir_event + (Name_t, Var_t) sync_event)``] derived_rules_deductionTheory.traces_def;
 val sbir_traces_t = (fst o strip_comb o fst o dest_eq o snd o strip_forall o concl) sbir_traces_thm;
 val sbir_traces_def = Define `
     sbir_traces = ^(sbir_traces_t)
 `;
     
 val DY_traces_thm =
-INST_TYPE [``:'symb`` |-> ``:Var_t``,``:'pred`` |-> ``:DYpred``,``:'state`` |-> ``:DYstate``,``:'event`` |-> ``:(DYnsyc_event + (Name_t, Var_t) sync_event)``] derived_rules_generaldeductionTheory.traces_def;
+INST_TYPE [``:'symb`` |-> ``:Var_t``,``:'pred`` |-> ``:DYpred``,``:'state`` |-> ``:DYstate``,``:'event`` |-> ``:(DYnsyc_event + (Name_t, Var_t) sync_event)``] derived_rules_deductionTheory.traces_def;
 val DY_traces_t = (fst o strip_comb o fst o dest_eq o snd o strip_forall o concl) DY_traces_thm;
 val DY_traces_def = Define `
     DY_traces = ^(DY_traces_t)
@@ -54,7 +54,7 @@ val bir_att_comptraces_def = Define `
 `;
 
 val sbir_DY_comptraces_thm =
-INST_TYPE [``:'symb`` |-> ``:Var_t``,``:'pred1`` |-> ``:'SPpred``,``:'state1`` |-> ``:(sbir_event, real,(bir_var_t, bir_exp_t) symb_interpret_t) stree``,``:'event1`` |-> ``:sbir_event``,``:'pred2`` |-> ``:DYpred``,``:'state2`` |-> ``:DYstate``,``:'event2`` |-> ``:DYnsyc_event``,``:'eventS`` |-> ``:(Name_t, Var_t) sync_event``] derived_rules_generaldeductionTheory.comptraces_def;
+INST_TYPE [``:'symb`` |-> ``:Var_t``,``:'pred1`` |-> ``:'SPpred``,``:'state1`` |-> ``:(sbir_event, real,(bir_var_t, bir_exp_t) symb_interpret_t) stree``,``:'event1`` |-> ``:sbir_event``,``:'pred2`` |-> ``:DYpred``,``:'state2`` |-> ``:DYstate``,``:'event2`` |-> ``:DYnsyc_event``,``:'eventS`` |-> ``:(Name_t, Var_t) sync_event``] derived_rules_deductionTheory.comptraces_def;
 val sbir_DY_comptraces_t = (fst o strip_comb o fst o dest_eq o snd o strip_forall o concl) sbir_DY_comptraces_thm;
 val sbir_DY_comptraces_def = Define `
     sbir_DY_comptraces = ^(sbir_DY_comptraces_t)
@@ -64,7 +64,7 @@ val sbir_DY_comptraces_def = Define `
 val compose_bir_attacker_vs_sbir_DY_thm = store_thm(
   "compose_bir_attacker_vs_sbir_DY_thm",
   ``
-  ∀(Sym:(Var_t -> bool)) (Sym':(Var_t -> bool)) (P:('SPpred + DYpred -> bool)) (P':('SPpred + DYpred -> bool)) (T0:(sbir_event, real,(bir_var_t, bir_exp_t) symb_interpret_t) stree) (Tre:(sbir_event, real,(bir_var_t, bir_exp_t) symb_interpret_t) stree) (birprog:'observation_type bir_program_t) (AMTrn:('attevent + 'ceventS, 'cstate) mctrel) (sbir_Ded:('SPpred) tded) (ded3:('SPpred + DYpred) tded).
+  ∀(Sym:(Var_t -> bool)) (Sym':(Var_t -> bool)) (P:('SPpred + DYpred -> bool)) (P':('SPpred + DYpred -> bool)) (T0:(sbir_event, real,(bir_var_t, bir_exp_t) symb_interpret_t) stree) (Tre:(sbir_event, real,(bir_var_t, bir_exp_t) symb_interpret_t) stree) (birprog:'observation_type bir_program_t) (AMTrn:('attevent + 'ceventS, 'cstate) mctrel) (sbir_Ded:('SPpred) tded).
 
         (
      (subset_one
@@ -76,10 +76,10 @@ val compose_bir_attacker_vs_sbir_DY_thm = store_thm(
 ) ==>
 (subset_comp
    (bir_att_comptraces (composeMuRe (((bir_mrel (birprog:'observation_type bir_program_t)): bir_state_t -> ('cevent + 'ceventS) list -> bir_state_t -> bool)) AMTrn) (((InterpretStOne:(sbir_event, real,(bir_var_t, bir_exp_t) symb_interpret_t) stree -> bir_state_t) T0),((InterpretStTwo:DYstate -> 'cstate) ESt)) (((InterpretStOne:(sbir_event, real,(bir_var_t, bir_exp_t) symb_interpret_t) stree -> bir_state_t) Tre),((InterpretStTwo:DYstate -> 'cstate) ESt)))
-   (sbir_DY_comptraces (symbolic_tree_multi_transitions_with_symb,sbir_Ded) (DYmultranrel,DYdeduction) ded3 (Sym,P,T0,ESt) (Sym',P',Tre,ESt))
+   (sbir_DY_comptraces (symbolic_tree_multi_transitions_with_symb,sbir_Ded) (DYmultranrel,DYdeduction) (Sym,P,T0,ESt) (Sym',P',Tre,ESt))
 )
 ``,
-rewrite_tac[interleavingconcreteTheory.binterleave_composition_concrete,binterleave_composition_generaldeduction,interleavingconcreteTheory.binterleave_ts,interleavinggeneraldeductionTheory.binterleave_ts,derived_rules_generaldeductionTheory.traces_def,interleavingconcreteTheory.traces_def,sbir_DY_comptraces_def,bir_att_comptraces_def,DY_traces_def,sbir_traces_def,att_traces_def,bir_traces_def]>>
+rewrite_tac[interleavingconcreteTheory.binterleave_composition_concrete,binterleave_composition_deduction,interleavingconcreteTheory.binterleave_ts,interleavingdeductionTheory.binterleave_ts,derived_rules_deductionTheory.traces_def,interleavingconcreteTheory.traces_def,sbir_DY_comptraces_def,bir_att_comptraces_def,DY_traces_def,sbir_traces_def,att_traces_def,bir_traces_def]>>
   FULL_SIMP_TAC (list_ss++pred_setSimps.PRED_SET_ss++boolSimps.LIFT_COND_ss++boolSimps.EQUIV_EXTRACT_ss) [subset_one_def,subset_two_def,subset_comp_def]>>
   rw[] >>
   PAT_X_ASSUM ``!x. A`` (ASSUME_TAC o (Q.SPECL [`((RevInterpretEvTwoSyn:('attevent + 'ceventS) list -> (DYnsyc_event + (Name_t, Var_t) sync_event) option list) (t2:(('attevent+'ceventS) list)))`]))>>
@@ -101,7 +101,7 @@ val birprog_def = Define `
 val compose_birexample_attacker_vs_sbir_DY_thm = store_thm(
   "compose_birexample_attacker_vs_sbir_DY_thm",
   ``
-  ∀(Sym:(Var_t -> bool)) (Sym':(Var_t -> bool)) (P:('SPpred + DYpred -> bool)) (P':('SPpred + DYpred -> bool)) (T0:(sbir_event, real,(bir_var_t, bir_exp_t) symb_interpret_t) stree) (Tre:(sbir_event, real,(bir_var_t, bir_exp_t) symb_interpret_t) stree) (AMTrn:('attevent + 'ceventS, 'cstate) mctrel) (sbir_Ded:('SPpred) tded) (ded3:('SPpred + DYpred) tded).
+  ∀(Sym:(Var_t -> bool)) (Sym':(Var_t -> bool)) (P:('SPpred + DYpred -> bool)) (P':('SPpred + DYpred -> bool)) (T0:(sbir_event, real,(bir_var_t, bir_exp_t) symb_interpret_t) stree) (Tre:(sbir_event, real,(bir_var_t, bir_exp_t) symb_interpret_t) stree) (AMTrn:('attevent + 'ceventS, 'cstate) mctrel) (sbir_Ded:('SPpred) tded).
 
         (
      (subset_one
@@ -113,7 +113,7 @@ val compose_birexample_attacker_vs_sbir_DY_thm = store_thm(
 ) ==>
 (subset_comp
    (bir_att_comptraces (composeMuRe (((bir_mrel (birprog:'observation_type bir_program_t)): bir_state_t -> ('cevent + 'ceventS) list -> bir_state_t -> bool)) AMTrn) (((InterpretStOne:(sbir_event, real,(bir_var_t, bir_exp_t) symb_interpret_t) stree -> bir_state_t) T0),((InterpretStTwo:DYstate -> 'cstate) ESt)) (((InterpretStOne:(sbir_event, real,(bir_var_t, bir_exp_t) symb_interpret_t) stree -> bir_state_t) Tre),((InterpretStTwo:DYstate -> 'cstate) ESt)))
-   (sbir_DY_comptraces (symbolic_tree_multi_transitions_with_symb,sbir_Ded) (DYmultranrel,DYdeduction) ded3 (Sym,P,T0,ESt) (Sym',P',Tre,ESt))
+   (sbir_DY_comptraces (symbolic_tree_multi_transitions_with_symb,sbir_Ded) (DYmultranrel,DYdeduction) (Sym,P,T0,ESt) (Sym',P',Tre,ESt))
 )
 ``,
 metis_tac[compose_bir_attacker_vs_sbir_DY_thm]
