HolBA/src/tools/parallelcomposition/DYLib/derived_rules_DYlibScript.sml
@@ -4,9 +4,9 @@ open pred_setTheory;
 open sigma_algebraTheory;
 open listTheory;
 open tautLib;
-open interleavinggeneraldeductionTheory;
-open parallelcompositiongeneraldeductionTheory;
-open derived_rules_generaldeductionTheory;
+open interleavingdeductionTheory;
+open parallelcompositiondeductionTheory;
+open derived_rules_deductionTheory;
 
 val _ = new_theory "derived_rules_DYlib";
 
@@ -21,22 +21,16 @@ val _ = Datatype `pred =
 Equal ('symb term) ('symb term)
       `;
 
-(* Sharing equalities *)        
-val composeDedEquSame_def =
-Define`
-      (composeDedEquSame (P3:((('symb) pred) + (('symb) pred)) set) ((INL ((Equal x y):(('symb) pred))):((('symb) pred) + (('symb) pred))) = (((Equal x y):(('symb) pred)) ∈ (IMAGE OUTR P3))) ∧
-(composeDedEquSame (P3:((('symb) pred) + (('symb) pred)) set) (INR ((Equal x y):(('symb) pred))) = (((Equal x y):(('symb) pred)) ∈ (IMAGE OUTL P3)))
-`;
 
 val same_function_signature_thm = store_thm(
   "same_function_signature_thm",
   ``!Sym Sym' P P' S1 S1' S2 S2' (MTrn1:(('event + 'eventS), ('symb pred), 'state, 'symb) mtrel) (Ded1:('symb pred) tded) (MTrn2:(('event + 'eventS), ('symb pred), 'state, 'symb) mtrel) (Ded2:('symb pred) tded).
-     (comptraces (MTrn1,Ded1) (MTrn2,Ded2) composeDedEquSame (Sym,P,S1,S2) (Sym',P',S1',S2'))                           
+     (comptraces (MTrn1,Ded1) (MTrn2,Ded2) (Sym,P,S1,S2) (Sym',P',S1',S2'))                           
   = (binterleave_ts (traces (MTrn1,Ded1) (Sym,(IMAGE OUTL P),S1) (Sym',(IMAGE OUTL P'),S1')) (traces (MTrn2,Ded2) (Sym,(IMAGE OUTR P),S2) (Sym',(IMAGE OUTR P'),S2')))
     ``,
   rewrite_tac[binterleave_ts,traces_def,comptraces_def,EXTENSION] >>
   rw[] >>
-  rewrite_tac[binterleave_trace_generaldeduction]
+  rewrite_tac[binterleave_trace_deduction]
   ); 
 
 
@@ -63,24 +57,18 @@ val _ = Datatype `predTwo =
 EqualTwo ('symb termTwo) ('symb termTwo)
          `;
 
-(* Sharing equalities *)
-val composeDedEquDistinct_def =
-Define`
-      (composeDedEquDistinct (P3:((('symb) predOne) + (('symb) predTwo)) set) ((INL ((EqualOne (NameOne x) (NameOne y)):(('symb) predOne))):((('symb) predOne) + (('symb) predTwo))) = (((EqualTwo (NameTwo x) (NameTwo y)):(('symb) predTwo)) ∈ (IMAGE OUTR P3))) ∧
-(composeDedEquDistinct (P3:((('symb) predOne) + (('symb) predTwo)) set) (INR ((EqualTwo (NameTwo x) (NameTwo y)):(('symb) predTwo))) = (((EqualOne (NameOne x) (NameOne y)):(('symb) predOne)) ∈ (IMAGE OUTL P3)))
-`;
 
 
 
 val distinct_function_signatures_thm = store_thm(
   "distinct_function_signatures_thm",
   ``∀Sym P S1 S2 Sym' P' S1' S2' (MTrn1:('event1 + 'eventS, ('symb predOne), 'state1, 'symb) mtrel) (MTrn2:('event2 + 'eventS, ('symb predTwo), 'state2, 'symb) mtrel) (Ded1:('symb predOne) tded) (Ded2:('symb predTwo) tded).
-         (comptraces (MTrn1,Ded1) (MTrn2,Ded2) composeDedEquDistinct (Sym,P,S1,S2) (Sym',P',S1',S2'))                           
+         (comptraces (MTrn1,Ded1) (MTrn2,Ded2) (Sym,P,S1,S2) (Sym',P',S1',S2'))                           
      = (binterleave_ts (traces (MTrn1,Ded1) (Sym,(IMAGE OUTL P),S1) (Sym',(IMAGE OUTL P'),S1')) (traces (MTrn2,Ded2) (Sym,(IMAGE OUTR P),S2) (Sym',(IMAGE OUTR P'),S2')))
        ``,
      rewrite_tac[binterleave_ts,traces_def,comptraces_def,EXTENSION] >>
      rw[] >>
-     rewrite_tac[binterleave_trace_generaldeduction]   
+     rewrite_tac[binterleave_trace_deduction]   
   ); 
 
 
