HolBA/src/tools/parallelcomposition/generaldeduction/derived_rules_generaldeductionScript.sml
@@ -24,12 +24,13 @@ Define`
 val binterleave_trace_comp_to_decomp_generaldeduction_thm = store_thm(
   "binterleave_trace_comp_to_decomp_generaldeduction",
   ``∀t Sym P S1 S2 Sym' P' S1' S2' (MTrn1:('event1 + 'eventS, 'pred1, 'state1, 'symb) mtrel) (MTrn2:('event2 + 'eventS, 'pred2, 'state2, 'symb) mtrel) (ded1:('pred1) tded) (ded2:('pred2) tded) (ded3:('pred1 + 'pred2) tded).
-       (symbolicParlComp (MTrn1,ded1) (MTrn2,ded2) ded3 (Sym,P,S1,S2) t (Sym',P',S1',S2'))
+       (TransEnable ded3 (MTrn1,ded1) (MTrn2,ded2)) ⇒
+       ((symbolicParlComp (MTrn1,ded1) (MTrn2,ded2) ded3 (Sym,P,S1,S2) t (Sym',P',S1',S2'))
      ⇒
      (∃t1 t2.
         (MTrn1 (Sym,(IMAGE OUTL P),S1) t1 (Sym',(IMAGE OUTL P'),S1')) ∧
         (MTrn2 (Sym,(IMAGE OUTR P),S2) t2 (Sym',(IMAGE OUTR P'),S2')) ∧
-        (binterl t1 t2 t))``,
+        (binterl t1 t2 t)))``,
                           GEN_TAC >>
      Induct_on `t` >- (
       FULL_SIMP_TAC (list_ss++pred_setSimps.PRED_SET_ss++boolSimps.LIFT_COND_ss++boolSimps.EQUIV_EXTRACT_ss)[symbolicParlComp_def]>>     
@@ -47,7 +48,7 @@ val binterleave_trace_comp_to_decomp_generaldeduction_thm = store_thm(
       Q.EXISTS_TAC `t1` >>
       Q.EXISTS_TAC `t2` >>
       FULL_SIMP_TAC (list_ss++pred_setSimps.PRED_SET_ss++boolSimps.LIFT_COND_ss++boolSimps.EQUIV_EXTRACT_ss)[]>>
-      metis_tac[DedRelAll,binterl_combinenone] 
+      metis_tac[TransEnable_def,binterl_combinenone] 
       )   >>
      Cases_on `x` >-(
       Cases_on `x'` >-(
@@ -89,22 +90,24 @@ val binterleave_trace_comp_to_decomp_generaldeduction_thm = store_thm(
 val binterleave_composition_generaldeduction_subseteq_thm = store_thm(
   "binterleave_composition_generaldeduction_subseteq",
   ``∀Sym P S1 S2 Sym' P' S1' S2' (MTrn1:('event1 + 'eventS, 'pred1, 'state1, 'symb) mtrel) (MTrn2:('event2 + 'eventS, 'pred2, 'state2, 'symb) mtrel) (Ded1:('pred1) tded) (Ded2:('pred2) tded) (ded3:('pred1 + 'pred2) tded).
-         (comptraces (MTrn1,Ded1) (MTrn2,Ded2) ded3 (Sym,P,S1,S2) (Sym',P',S1',S2'))                           
-      ⊆ (binterleave_ts (traces (MTrn1,Ded1) (Sym,(IMAGE OUTL P),S1) (Sym',(IMAGE OUTL P'),S1')) (traces (MTrn2,Ded2) (Sym,(IMAGE OUTR P),S2) (Sym',(IMAGE OUTR P'),S2')))
+         (TransEnable ded3 (MTrn1,Ded1) (MTrn2,Ded2)) ⇒
+         ((comptraces (MTrn1,Ded1) (MTrn2,Ded2) ded3 (Sym,P,S1,S2) (Sym',P',S1',S2'))                           
+      ⊆ (binterleave_ts (traces (MTrn1,Ded1) (Sym,(IMAGE OUTL P),S1) (Sym',(IMAGE OUTL P'),S1')) (traces (MTrn2,Ded2) (Sym,(IMAGE OUTR P),S2) (Sym',(IMAGE OUTR P'),S2'))))
        ``,
        rpt gen_tac >>      
      rewrite_tac[binterleave_ts,traces_def,comptraces_def,EXTENSION] >>
      FULL_SIMP_TAC (list_ss++pred_setSimps.PRED_SET_ss++boolSimps.LIFT_COND_ss++boolSimps.EQUIV_EXTRACT_ss) [SUBSET_DEF] >>
-     rewrite_tac[binterleave_trace_comp_to_decomp_generaldeduction_thm]   
+     metis_tac[binterleave_trace_comp_to_decomp_generaldeduction_thm]   
   );
 
   
 val binterleave_trace_decomp_to_comp_generaldeduction_thm = store_thm(
   "binterleave_trace_decomp_to_comp_generaldeduction",
   ``∀t Sym P S1 S2 Sym' P' S1' S2' (MTrn1:('event1 + 'eventS, 'pred1, 'state1, 'symb) mtrel) (MTrn2:('event2 + 'eventS, 'pred2, 'state2, 'symb) mtrel) (ded1:('pred1) tded) (ded2:('pred2) tded) (ded3:('pred1 + 'pred2) tded). 
-       (∃t1 t2. (MTrn1 (Sym,(IMAGE OUTL P),S1) t1 (Sym',(IMAGE OUTL P'),S1')) ∧ (MTrn2 (Sym,(IMAGE OUTR P),S2) t2 (Sym',(IMAGE OUTR P'),S2')) ∧ (binterl t1 t2 t))
+       TransDisable ded3 (MTrn1,ded1) (MTrn2,ded2) ⇒
+       ((∃t1 t2. (MTrn1 (Sym,(IMAGE OUTL P),S1) t1 (Sym',(IMAGE OUTL P'),S1')) ∧ (MTrn2 (Sym,(IMAGE OUTR P),S2) t2 (Sym',(IMAGE OUTR P'),S2')) ∧ (binterl t1 t2 t))
      ⇒
-     (symbolicParlComp (MTrn1,ded1) (MTrn2,ded2) ded3 (Sym,P,S1,S2) t (Sym',P',S1',S2'))
+     (symbolicParlComp (MTrn1,ded1) (MTrn2,ded2) ded3 (Sym,P,S1,S2) t (Sym',P',S1',S2')))
      ``,
      GEN_TAC >>
      Induct_on `t` >-
@@ -182,71 +185,44 @@ val binterleave_trace_decomp_to_comp_generaldeduction_thm = store_thm(
      Q.EXISTS_TAC `P''` >>
      PAT_X_ASSUM ``!Ded1 Ded2 Ded3. A`` (ASSUME_TAC o (Q.SPECL [`ded1`,`ded2`,`ded3`]))  >>
      PAT_X_ASSUM ``!Ded1 Ded2 Ded3. A`` (ASSUME_TAC o (Q.SPECL [`ded1`,`ded2`,`ded3`]))  >>
-     rw[] 
+     rw[TransDisable_def] 
   );
 
 
 val binterleave_composition_generaldeduction_supseteq_thm = store_thm(
   "binterleave_composition_generaldeduction_supseteq",
   ``∀Sym P S1 S2 Sym' P' S1' S2' (MTrn1:('event1 + 'eventS, 'pred1, 'state1, 'symb) mtrel) (MTrn2:('event2 + 'eventS, 'pred2, 'state2, 'symb) mtrel) (Ded1:('pred1) tded) (Ded2:('pred2) tded) (ded3:('pred1 + 'pred2) tded).
-         (binterleave_ts (traces (MTrn1,Ded1) (Sym,(IMAGE OUTL P),S1) (Sym',(IMAGE OUTL P'),S1')) (traces (MTrn2,Ded2) (Sym,(IMAGE OUTR P),S2) (Sym',(IMAGE OUTR P'),S2'))) ⊆
-         (comptraces (MTrn1,Ded1) (MTrn2,Ded2) ded3 (Sym,P,S1,S2) (Sym',P',S1',S2'))
+         TransDisable ded3 (MTrn1,Ded1) (MTrn2,Ded2) ⇒
+         ((binterleave_ts (traces (MTrn1,Ded1) (Sym,(IMAGE OUTL P),S1) (Sym',(IMAGE OUTL P'),S1')) (traces (MTrn2,Ded2) (Sym,(IMAGE OUTR P),S2) (Sym',(IMAGE OUTR P'),S2'))) ⊆
+         (comptraces (MTrn1,Ded1) (MTrn2,Ded2) ded3 (Sym,P,S1,S2) (Sym',P',S1',S2')))
        ``,
          rpt gen_tac >>      
      rewrite_tac[binterleave_ts,traces_def,comptraces_def,EXTENSION] >>
      FULL_SIMP_TAC (list_ss++pred_setSimps.PRED_SET_ss++boolSimps.LIFT_COND_ss++boolSimps.EQUIV_EXTRACT_ss) [SUBSET_DEF] >>
-     rewrite_tac[binterleave_trace_decomp_to_comp_generaldeduction_thm]     
+     metis_tac[binterleave_trace_decomp_to_comp_generaldeduction_thm]     
   );
   
-  
-val binterleave_trace_generaldeduction_thm = store_thm(
-  "binterleave_trace_generaldeduction",
-  `` ∀t Sym P S1 S2 Sym' P' S1' S2' (MTrn1:('event1 + 'eventS, 'pred1, 'state1, 'symb) mtrel) (MTrn2:('event2 + 'eventS, 'pred2, 'state2, 'symb) mtrel) (ded1:('pred1) tded) (ded2:('pred2) tded) (ded3:('pred1 + 'pred2) tded). 
-       (symbolicParlComp (MTrn1,ded1) (MTrn2,ded2) ded3 (Sym,P,S1,S2) t (Sym',P',S1',S2'))
-       ⇔
-         (∃t1 t2. (MTrn1 (Sym,(IMAGE OUTL P),S1) t1 (Sym',(IMAGE OUTL P'),S1')) ∧ (MTrn2 (Sym,(IMAGE OUTR P),S2) t2 (Sym',(IMAGE OUTR P'),S2')) ∧ (binterl t1 t2 t))
-         ``,
-  rpt gen_tac >>
-  EQ_TAC >>
-  rewrite_tac[binterleave_trace_comp_to_decomp_generaldeduction_thm] >>
-  rewrite_tac[binterleave_trace_decomp_to_comp_generaldeduction_thm]
-  );
+ 
 
-val binterleave_composition_generaldeduction_thm = store_thm(
-  "binterleave_composition_generaldeduction",
-  ``∀Sym P S1 S2 Sym' P' S1' S2' (MTrn1:('event1 + 'eventS, 'pred1, 'state1, 'symb) mtrel) (MTrn2:('event2 + 'eventS, 'pred2, 'state2, 'symb) mtrel) (Ded1:('pred1) tded) (Ded2:('pred2) tded) (ded3:('pred1 + 'pred2) tded).
-         (comptraces (MTrn1,Ded1) (MTrn2,Ded2) ded3 (Sym,P,S1,S2) (Sym',P',S1',S2'))                           
-     = (binterleave_ts (traces (MTrn1,Ded1) (Sym,(IMAGE OUTL P),S1) (Sym',(IMAGE OUTL P'),S1')) (traces (MTrn2,Ded2) (Sym,(IMAGE OUTR P),S2) (Sym',(IMAGE OUTR P'),S2')))
-       ``,
-       rewrite_tac[SET_EQ_SUBSET,binterleave_composition_generaldeduction_supseteq_thm,binterleave_composition_generaldeduction_subseteq_thm]
-  ); 
-
-
-val compose_vs_modules_generaldeduction_thm = store_thm(
-  "compose_vs_modules_generaldeduction_thm",
+val compose_vs_modules_generaldeduction_enable_disable_thm = store_thm(
+  "compose_vs_modules_generaldeduction_enable_disable_thm",
   ``!Sym Sym' Sym'' Sym''' P P' P'' P''' S1 S1' S1'' S1''' S2 S2' S2'' S2''' (MTrn1:('event1 + 'eventS, 'pred1, 'state1, 'symb) mtrel) (MTrn1':('event1 + 'eventS, 'pred1, 'state1, 'symb) mtrel) (MTrn2:('event2 + 'eventS, 'pred2, 'state2, 'symb) mtrel) (MTrn2':('event2 + 'eventS, 'pred2, 'state2, 'symb) mtrel) (Ded1:('pred1) tded) (Ded1':('pred1) tded) (Ded2:('pred2) tded) (Ded2':('pred2) tded) (ded3:('pred1 + 'pred2) tded).
-     (((traces (MTrn1,Ded1) (Sym,(IMAGE OUTL P),S1) (Sym',(IMAGE OUTL P'),S1')) ⊆ (traces (MTrn1',Ded1') (Sym'',(IMAGE OUTL P''),S1'') (Sym''',(IMAGE OUTL P'''),S1'''))) ∧ ((traces (MTrn2,Ded2) (Sym,(IMAGE OUTR P),S2) (Sym',(IMAGE OUTR P'),S2')) ⊆ (traces (MTrn2',Ded2') (Sym'',(IMAGE OUTR P''),S2'') (Sym''',(IMAGE OUTR P'''),S2''')))
-     ) ==> ((comptraces (MTrn1,Ded1) (MTrn2,Ded2) ded3 (Sym,P,S1,S2) (Sym',P',S1',S2')) ⊆ (comptraces (MTrn1',Ded1') (MTrn2',Ded2') ded3 (Sym'',P'',S1'',S2'') (Sym''',P''',S1''',S2'''))) ``
+     (((traces (MTrn1,Ded1) (Sym,(IMAGE OUTL P),S1) (Sym',(IMAGE OUTL P'),S1')) ⊆ (traces (MTrn1',Ded1') (Sym'',(IMAGE OUTL P''),S1'') (Sym''',(IMAGE OUTL P'''),S1'''))) ∧
+      ((traces (MTrn2,Ded2) (Sym,(IMAGE OUTR P),S2) (Sym',(IMAGE OUTR P'),S2')) ⊆ (traces (MTrn2',Ded2') (Sym'',(IMAGE OUTR P''),S2'') (Sym''',(IMAGE OUTR P'''),S2'''))) ∧
+      (TransEnable ded3 (MTrn1,Ded1) (MTrn2,Ded2)) ∧
+      (TransDisable ded3 (MTrn1',Ded1') (MTrn2',Ded2'))
+ ) ==> ((comptraces (MTrn1,Ded1) (MTrn2,Ded2) ded3 (Sym,P,S1,S2) (Sym',P',S1',S2')) ⊆ (comptraces (MTrn1',Ded1') (MTrn2',Ded2') ded3 (Sym'',P'',S1'',S2'') (Sym''',P''',S1''',S2'''))) ``
   ,
 rpt gen_tac >>      
 rewrite_tac[binterleave_ts,traces_def,comptraces_def,EXTENSION] >>
 FULL_SIMP_TAC (list_ss++pred_setSimps.PRED_SET_ss++boolSimps.LIFT_COND_ss++boolSimps.EQUIV_EXTRACT_ss) [SUBSET_DEF] >>
-metis_tac[binterleave_trace_comp_to_decomp_generaldeduction_thm,binterleave_trace_decomp_to_comp_generaldeduction_thm]
+rw[] >>
+IMP_RES_TAC binterleave_trace_comp_to_decomp_generaldeduction_thm >>
+PAT_X_ASSUM ``!t2. A`` (ASSUME_TAC o (Q.SPECL [`t2`])) >>
+PAT_X_ASSUM ``!t1. A`` (ASSUME_TAC o (Q.SPECL [`t1`])) >>
+RES_TAC >>
+metis_tac[binterleave_trace_decomp_to_comp_generaldeduction_thm]
   );  
-
-
-
-
-
-
-
-
-
-
-
-
-
-
 
 
 
