HolBA/src/tools/parallelcomposition/instantiations/sbir_sapic_comp_DYScript.sml
@@ -4,10 +4,10 @@ open pred_setTheory;
 open sigma_algebraTheory;
 open listTheory;
 open tautLib;
-open interleavinggeneraldeductionTheory;
-open parallelcompositiongeneraldeductionTheory;
+open interleavingdeductionTheory;
+open parallelcompositiondeductionTheory;
 open translate_to_sapicTheory;
-open derived_rules_generaldeductionTheory;
+open derived_rules_deductionTheory;
 open sbir_treeTheory;
 open sapicplusTheory;
 open messagesTheory;
@@ -20,12 +20,11 @@ Define`
       comptraces_sapic
       ((MTrn1:(SapicFact_t + (Name_t,Var_t) sync_event, 'SPpred, sapic_position_configuration_t, Var_t) mtrel),(Ded1:('SPpred) tded))
       ((MTrn2:(DYnsyc_event + (Name_t,Var_t) sync_event, DYpred, DYstate, Var_t) mtrel),(Ded2:(DYpred) tded))
-      (ded3:('SPpred + DYpred) tded)
       ((Sym:Var_t set),(P: ('SPpred + DYpred) set),(S1: sapic_position_configuration_t),(S2: DYstate))
       ((Sym':Var_t set),(P': ('SPpred + DYpred) set),(S1': sapic_position_configuration_t),(S2': DYstate))
 =
 {(t:((SapicFact_t + (Name_t,Var_t) sync_event)+(DYnsyc_event + (Name_t,Var_t) sync_event)) option list)|  
- (symbolicParlComp (MTrn1,Ded1) (MTrn2,Ded2) ded3 (Sym,P,S1,S2) t (Sym',P',S1',S2'))
+ (symbolicParlComp (MTrn1,Ded1) (MTrn2,Ded2) (Sym,P,S1,S2) t (Sym',P',S1',S2'))
 }
 `;
 
@@ -34,12 +33,11 @@ Define`
       comptraces_tree
       ((MTrn1:((sbir_event + (Name_t, Var_t) sync_event), 'SPpred, (sbir_event, real,(bir_var_t, bir_exp_t) symb_interpret_t) stree, Var_t) mtrel),(Ded1:('SPpred) tded))
       ((MTrn2:(DYnsyc_event + (Name_t,Var_t) sync_event, DYpred, DYstate, Var_t) mtrel),(Ded2:(DYpred) tded))
-      (ded3:('SPpred + DYpred) tded)
       ((Sym:Var_t set),(P: ('SPpred + DYpred) set),(S1: (sbir_event, real,(bir_var_t, bir_exp_t) symb_interpret_t) stree),(S2: DYstate))
       ((Sym':Var_t set),(P': ('SPpred + DYpred) set),(S1': (sbir_event, real,(bir_var_t, bir_exp_t) symb_interpret_t) stree),(S2': DYstate))
 =
 {(t: (((sbir_event + (Name_t, Var_t) sync_event) + DYnsyc_event + (Name_t,Var_t) sync_event) option list))|  
- (symbolicParlComp (MTrn1,Ded1) (MTrn2,Ded2) ded3 (Sym,P,S1,S2) t (Sym',P',S1',S2'))
+ (symbolicParlComp (MTrn1,Ded1) (MTrn2,Ded2) (Sym,P,S1,S2) t (Sym',P',S1',S2'))
 }
 `;
 
@@ -121,10 +119,10 @@ val compose_sbir_sapic_vs_DY_thm = store_thm(
   ``∀T0 Re0 NRe0 i Re NRe Tre (Sym:(Var_t -> bool)) (Sym':(Var_t -> bool)) (P:('SPpred + DYpred -> bool)) (P':('SPpred + DYpred -> bool)) (Ded:('SPpred) tded) (ded3:('SPpred + DYpred) tded).
         ((IMAGE (MAP sbirEvent_vs_Sync_to_sapicFact_vs_Sync) (traces_of_tree_with_symb (Sym,IMAGE OUTL P,T0) (Sym',IMAGE OUTL P',Tre))) ⊆ (traces_of_sapic_with_symb (Sym,IMAGE OUTL P,(Pconfig ((symbtree_to_sapic T0),0,Re0,NRe0))) (Sym',IMAGE OUTL P',(Pconfig ((symbtree_to_sapic Tre),i,Re,NRe)))))
      ==> (
-      (IMAGE (MAP sbirEvent_vs_DY_to_sapicFact_vs_DY) (comptraces_tree (symbolic_tree_multi_transitions_with_symb,Ded) (DYmultranrel,DYdeduction) ded3 (Sym,P,T0,ESt) (Sym',P',Tre,ESt))) ⊆
-      (comptraces_sapic (sapic_position_multi_transitions_with_symb,Ded) (DYmultranrel,DYdeduction) ded3 (Sym,P,(Pconfig ((symbtree_to_sapic T0),0,Re0,NRe0)),ESt) (Sym',P',(Pconfig ((symbtree_to_sapic Tre),i,Re,NRe)),ESt))
+      (IMAGE (MAP sbirEvent_vs_DY_to_sapicFact_vs_DY) (comptraces_tree (symbolic_tree_multi_transitions_with_symb,Ded) (DYmultranrel,DYdeduction) (Sym,P,T0,ESt) (Sym',P',Tre,ESt))) ⊆
+      (comptraces_sapic (sapic_position_multi_transitions_with_symb,Ded) (DYmultranrel,DYdeduction) (Sym,P,(Pconfig ((symbtree_to_sapic T0),0,Re0,NRe0)),ESt) (Sym',P',(Pconfig ((symbtree_to_sapic Tre),i,Re,NRe)),ESt))
       ) ``,
-        FULL_SIMP_TAC (list_ss++pred_setSimps.PRED_SET_ss++boolSimps.LIFT_COND_ss++boolSimps.EQUIV_EXTRACT_ss) [traces_of_tree_with_symb_def,traces_of_sapic_with_symb_def,EXTENSION,SUBSET_DEF,comptraces_tree_def, comptraces_sapic_def,binterleave_composition_generaldeduction,binterleave_ts,binterleave_trace_generaldeduction] >>    
+        FULL_SIMP_TAC (list_ss++pred_setSimps.PRED_SET_ss++boolSimps.LIFT_COND_ss++boolSimps.EQUIV_EXTRACT_ss) [traces_of_tree_with_symb_def,traces_of_sapic_with_symb_def,EXTENSION,SUBSET_DEF,comptraces_tree_def, comptraces_sapic_def,binterleave_composition_deduction,binterleave_ts,binterleave_trace_deduction] >>    
      rpt strip_tac >>
      PAT_X_ASSUM ``!x. A`` (ASSUME_TAC o (Q.SPECL [`(MAP sbirEvent_vs_Sync_to_sapicFact_vs_Sync t1)`])) >>
      RES_TAC  >>
